improve performance to make not-totally-trivial examples work
* Order `Proper` constraints first because `Subrel` goes into a lot more
  of a speculative frenzy than `Proper` does.
* Reorder some hints in the `grewrite` database to solve a bit quicker.
  (Hints are not yet ordered by "cost").
* Sort instances by cost, although that cost is currently meh.
* Finally some non-trivial examples work.

GeneralizedRewriting/Defs.lean
@@ -23,9 +23,6 @@ class PER {α: Type _} (R: relation α) extends Symmetric R, Transitive R
 
 class Equiv {α: Type _} (R: relation α) extends PER R, Reflexive R
 
-eauto_create_db grewrite
-eauto_hint Reflexive.refl: grewrite
-
 /-
 ## Morphisms
 -/
@@ -54,20 +51,26 @@ notation Rα " ==> " Rβ => respectful Rα Rβ
 
 -- Instances used by the search algorithm
 
-instance Reflexive_Subrel: Reflexive (@Subrel α) where
-  refl _ := ⟨id⟩
+-- Avoid a `Reflexive (@Subrel α)` instance because that would allow `Subrel`
+-- to be guessed as a codomain relation without an explicit hint, which almost
+-- never makes sense.
+theorem Reflexive_Subrel (R: relation α): Subrel R R := ⟨id⟩
 
 instance Subrel_respectful [Sα: @Subrel α R₂ R₁] [Sβ: @Subrel β S₁ S₂]:
     Subrel (R₁ ==> S₁) (R₂ ==> S₂) where
   prf H _ _ h := Sβ.prf (H _ _ (Sα.prf h))
 
+instance Subrel_pointwise [S: @Subrel β R₁ R₂]:
+    Subrel (pointwise_relation α R₁) (pointwise_relation α R₂) where
+  prf h a := S.prf (h a)
+
 instance Proper_pointwise_relation {α β: Type _}:
     Proper (Subrel ==> Subrel) (@pointwise_relation α β) where
   prf _ _ h := ⟨fun hpr a => h.prf (hpr a)⟩
 
-instance Subrel_pointwise [S: @Subrel β R₁ R₂]:
-    Subrel (pointwise_relation α R₁) (pointwise_relation α R₂) where
-  prf h a := S.prf (h a)
+instance Proper_Reflexive {α: Type _} (Rα: relation α) [Reflexive Rα] (a: α):
+    Proper Rα a where
+  prf := Reflexive.refl _
 
 -- Standard instances
 
@@ -103,6 +106,9 @@ instance Subrel_Iff_flip_impl: Subrel Iff (flip impl) where
 
 --
 
+-- TODO: We can assume `Transitive R` and instead put `flip` in judicious
+-- places for these rules. (This might require better suport for `flip`.)
+
 instance {R: relation α} [PER R]: Proper (R ==> R ==> Iff) R where
   prf _ _ h_a _ _ h_b :=
     ⟨fun h => Transitive.trans (Transitive.trans (Symmetric.symm h_a) h) h_b,
@@ -118,45 +124,7 @@ instance {R: relation α} [PER R]: Proper (Eq ==> R ==> Iff) R where
     ⟨by rewrite [h_a]; exact fun h => Transitive.trans h h_b,
      by rewrite [h_a]; exact fun h => Transitive.trans h (Symmetric.symm h_b)⟩
 
-section Examples
-
-variable (α β γ: Type)
-variable (Rα: relation α) (Rβ: relation β) (Rγ: relation γ)
-variable [PER Rα] [PER Rβ] [PER Rγ]
-variable (Pα: α → Prop) (Pβ: β → Prop) (Pγ: γ → Prop)
-variable (Pαβγ: α → β → Prop)
-variable (fαβ: α → β) (fβγ: β → γ)
-variable [Proper_fαβ: Proper (Rα ==> Rβ) fαβ]
-
-example (h: Rα a a'): Rβ (fαβ a) x := by
-  -- We want to rewrite `h: Rα a a'`.
-  -- The TERM to rewrite is `a`. The RELATION is `Rα`.
-
-  -- Start at the targeted occurrence of the TERM to rewrite (here `a`). Move
-  -- up to the root of the term.
-
-  -- When an application is encountered, build a `Proper` instance for it:
-  -- * The argument position where the TERM to rewrite is: use the RELATION
-  -- * All other arguments: use `Eq`
-  -- * Output: guess it and/or see what typeclass search comes up with
-  --   (here `Rβ`)
-  -- Note there are many unadressed questions about how to discover the
-  -- instance, including dealing with subrelations etc.
-  have P₁: Proper (Rα ==> Rβ) fαβ := inferInstance
-  -- Apply that instance:
-  -- * For each argument left untouched, apply `_ _ rfl`
-  -- * For the argument being changed, apply `_ _ h`
-  have h₁: Rβ (fαβ a) (fαβ a') := P₁.prf _ _ h
-
-  -- Then proceed upwards, replacing `h` with `h₁`, the TERM to rewrite with
-  -- the call where it's located (here `fαβ a`), and the RELATION with whatever
-  -- has been found (here `Rβ`).
-
-  -- When reaching the top-level, if the goal is of sort `Prop`, finish with
-  -- `Iff`, otherwise finish with `Eq`.
-  have P₂: Proper (Rβ ==> Eq ==> Iff) Rβ := inferInstance
-  have h₂: Iff (Rβ (fαβ a) x) (Rβ (fαβ a') x) := P₂.prf _ _ h₁ _ _ rfl
-
-  rewrite [h₂]
-  sorry
-end Examples
+-- Order the hints by most specific first
+eauto_create_db grewrite
+eauto_hint Reflexive_Subrel: grewrite
+eauto_hint Reflexive.refl: grewrite
