GeneralizedRewriting.lean
@@ -1,2 +1,7 @@
 import GeneralizedRewriting.Defs
 import GeneralizedRewriting.Algorithm
+import GeneralizedRewriting.Eauto
+
+-- As a check that examples pass
+import GeneralizedRewriting.TestsEauto
+import GeneralizedRewriting.TestsGrewrite
